src/axiomatic/SimInitial.v
@@ -1,0 +1,117 @@
+(******************************************************************************)
+(** * Simulation between initial states  *)
+(******************************************************************************)
+
+Require Import Classical List Relations Peano_dec.
+Require Import Hahn.
+Require Import sflib.
+Require Import paco.
+
+Require Import Axioms.
+Require Import Basic.
+Require Import Language.
+Require Import Event.
+Require Import Time.
+Require Import Configuration.
+Require Import View.
+Require Import Cell.
+Require Import Memory.
+Require Import Thread.
+Require Import TView.
+
+Require Import Gevents.
+Require Import model.
+Require Import Machine.
+Require Import SimRel.
+
+Set Implicit Arguments.
+Remove Hints plus_n_O.
+
+Require Import Setoid Permutation.
+
+Lemma coherent_initial G (INIT: initial_exec G) : 
+  Coherent (acts G) (sb G) (rmw G) (rf G) (mo G) (sc G).
+Proof.
+destruct INIT; red; splits; red; splits; try red; splits; ins; eauto.
+all: try by specialize (ACTS a); tauto.
+all: try by exfalso; specialize (SB a b); tauto.
+all: try by exfalso; specialize (RMW a b); tauto.
+all: try by exfalso; specialize (RF a b); tauto.
+all: try by exfalso; specialize (RF a c); tauto.
+all: try by exfalso; specialize (MO a b); tauto.
+all: try by exfalso; specialize (SC a b); tauto.
+by unfold init_pair in *; desc; eapply proper_non_init in INIT0; 
+specialize (ACTS b); tauto.
+by intro; ins; eapply SB; eauto.
+by intro; ins; exfalso; eapply SB; eauto.
+by exfalso; eapply proper_non_init in PROPERa; specialize (ACTS a); tauto.
+{ apply read_non_write in READ.
+  assert (is_init b -> is_write b).
+  by eapply init_is_write.
+  specialize (ACTS b).
+  tauto. }
+by intro; ins; eapply MO; eauto.
+by intro; ins; exfalso; eapply MO; eauto.
+{ intro; ins; desc.
+  exfalso.
+  apply NEQ.
+  apply same_init.
+  specialize (ACTS a); tauto.
+  specialize (ACTS b); tauto.
+  congruence. }
+by intro; ins; eapply SC; eauto.
+by intro; ins; exfalso; eapply SC; eauto.
+{ intro; ins; desc.
+  apply ACTS, init_not_sc in IWa.
+  exfalso; eauto with acts. }
+{ intros x H. apply t_step_rt in H; desc.
+  unfold Relation_Operators.union in H; desf; exfalso.
+  specialize (SB x z); tauto.
+  specialize (RF x z); tauto.
+  specialize (SC x z); tauto. }
+Qed.
+
+Lemma sim_initial :
+  forall s ax_st (INIT: initial ax_st s),
+    GMsim (Configuration.init s) ax_st.
+Proof.
+ins.
+destruct INIT.
+red; splits.
+- by apply coherent_initial.
+- apply Configuration.init_wf.
+- ins. unfold Threads.init in *.
+  apply find_mapD in TID; desc.
+  desf.
+- admit.
+- eexists _,_.
+red; splits.
+* red; ins; exfalso.
+destruct EXEC; desc.
+eapply MO; edone.
+* ins.
+unfold Threads.init in *.
+  apply find_mapD in TID; desf.
+unfold Local.init in *; ins.
+red; splits; red; splits; ins.
+all: eapply max_value_empty.
+all: ins; intro H.
+all: unfold t_cur, t_acq, t_rel, dom_rel, c_cur, c_acq, c_rel, seq, eqv_rel in *; desc.
+(* + 
+eapply urr_actb in H; eauto using coherent_initial.
+
+destruct EXEC.
+apply ACTS in H.
+red in H.
+unfold init_event in *.
+desc; destruct y as [??[]]; ins; desf.
++ 
+red in H.
+red in H.
+desc.
+red in H.
+ *)
+(* 
+unfold  *)
+all: admit.
+Admitted.
